Abstract RSC_DC_MD (and 3): Intermediate
See comments for some technical information. Source currently presents a
dependency on Intermediate, which is probably extraneous and should
eventually be moved out, thus simplifying the nestings.

Some local changes to the top-level proof were needed beyond the usual
addition and correction of qualified module names, due to its local
reliance on low-level tactics manipulating entities of the concrete
Intermediate. For this reason the abstract interface has to be extended
with some additional exposed definitions and inversion lemmas, which
correspond to trivial proofs in the instantiation of the module
signature with the concrete instance.

The proof is now generic modulo the Common and CompCert infrastructure.

RSC_DC_MD.v
@@ -28,7 +28,18 @@ Set Bullet Behavior "Strict Subproofs".
    the high-level proof here.
 
    The repetition verbatim of theorem statements as axioms is particularly
-   annoying; we will want to eliminate this duplication. *)
+   annoying; we will want to eliminate this duplication.
+
+   Note the blame lemma in Source as a dependency on Intermediate. Should
+   we keep it this way? It feels ugly.
+
+   Naming comventions can also be harmonized.
+
+   The current proof is generic while still relying on our Common and
+   CompCert's infrastructure. Note that PS.mergeable_interfaces is defined
+   in Intermediate and used there, but is actually independent from it and
+   not factored as part of the interface: this points to it belonging in
+   Common and not in Intermediate. *)
 
 Module Type Intermediate_Sig.
   Parameter program : Type.
@@ -43,6 +54,27 @@ Module Type Intermediate_Sig.
 
   Parameter program_link : program -> program -> program.
 
+  Axiom program_linkC : forall p1 p2,
+    well_formed_program p1 ->
+    well_formed_program p2 ->
+    linkable (prog_interface p1) (prog_interface p2) ->
+    program_link p1 p2 = program_link p2 p1.
+
+  Axiom linking_well_formedness : forall p1 p2,
+    well_formed_program p1 ->
+    well_formed_program p2 ->
+    linkable (prog_interface p1) (prog_interface p2) ->
+    well_formed_program (program_link p1 p2).
+
+  Axiom interface_preserves_closedness_r : forall p1 p2 p2',
+    well_formed_program p1 ->
+    well_formed_program p2' ->
+    prog_interface p2 = prog_interface p2' ->
+    linkable (prog_interface p1) (prog_interface p2) ->
+    closed_program (program_link p1 p2) ->
+    linkable_mains p1 p2 ->
+    closed_program (program_link p1 p2').
+
   Module CS.
     Parameter sem : program -> semantics.
   End CS.
@@ -50,9 +82,67 @@ Module Type Intermediate_Sig.
   Module PS.
     Parameter sem : program -> Program.interface -> semantics.
   End PS.
+
+  Axiom decomposition_with_safe_behavior:
+    forall p c,
+      well_formed_program p ->
+      well_formed_program c ->
+      linkable (prog_interface p) (prog_interface c) ->
+    forall beh,
+      program_behaves (CS.sem (program_link p c)) beh ->
+      not_wrong beh ->
+      program_behaves (PS.sem p (prog_interface c)) beh.
+
+  Axiom decomposition_with_refinement :
+    forall p c,
+      well_formed_program p ->
+      well_formed_program c ->
+      linkable (prog_interface p) (prog_interface c) ->
+    forall beh1,
+      program_behaves (CS.sem (program_link p c)) beh1 ->
+    exists beh2,
+      program_behaves (PS.sem p (prog_interface c)) beh2 /\
+      behavior_improves beh1 beh2.
+
+  Axiom composition_prefix :
+    forall p c,
+      well_formed_program p ->
+      well_formed_program c ->
+      linkable_mains p c ->
+      linkable (prog_interface p) (prog_interface c) ->
+      closed_program (program_link p c) ->
+      PS.mergeable_interfaces (prog_interface p) (prog_interface c) ->
+    forall b1 b2 m,
+      program_behaves (PS.sem p (prog_interface c)) b1 ->
+      program_behaves (PS.sem c (prog_interface p)) b2 ->
+      prefix m b1 ->
+      prefix m b2 ->
+    exists b3,
+      program_behaves (CS.sem (program_link p c)) b3 /\ prefix m b3.
+
+  (* The top-level proof performs low-level manipulations on the now-abstract
+     definitions in a couple of places. These definitions must now become
+     opaque and exposed through the interface, and its operations given as
+     trivial inversion-type lemmas. We may want to think about removing these
+     noisy details through further abstraction. *)
+  Parameter prog_main : program -> option Procedure.id.
+
+  Parameter prog_procedures : program -> NMap (NMap code).
+
+  Axiom closed_program_inv : forall p,
+    closed_program p ->
+    closed_interface (prog_interface p) /\
+    exists mainP main_procs,
+      prog_main p = Some mainP /\
+      (prog_procedures p) Component.main = Some main_procs /\
+      mainP \in domm main_procs.
+
+  Axiom closed_interface_inv : forall p1 p2,
+    closed_interface (prog_interface (program_link p1 p2)) =
+    closed_interface (unionm (prog_interface p1) (prog_interface p2)).
 End Intermediate_Sig.
 
-Module Intermediate_Instace : Intermediate_Sig.
+Module Intermediate_Instance <: Intermediate_Sig.
   Definition program :=
     @Intermediate.program.
 
@@ -71,6 +161,15 @@ Module Intermediate_Instace : Intermediate_Sig.
   Definition program_link :=
     @Intermediate.program_link.
 
+  Definition program_linkC :=
+    @Intermediate.program_linkC.
+
+  Definition linking_well_formedness :=
+    @Intermediate.linking_well_formedness.
+
+  Definition interface_preserves_closedness_r :=
+    @Intermediate.interface_preserves_closedness_r.
+
   Module CS.
     Definition sem :=
       @Intermediate.CS.CS.sem.
@@ -79,11 +178,48 @@ Module Intermediate_Instace : Intermediate_Sig.
   Module PS.
     Definition sem :=
       @Intermediate.PS.PS.sem.
-  End PS.  
-End Intermediate_Instace.
+    End PS.
 
+  Definition decomposition_with_safe_behavior :=
+    @Intermediate.Decomposition.decomposition_with_safe_behavior.
 
-Module Type Source_Sig.
+  Definition decomposition_with_refinement :=
+    @Intermediate.Decomposition.decomposition_with_refinement.
+
+  Definition composition_prefix :=
+    @Intermediate.Composition.composition_prefix.
+
+  (* The following additions are required by the top-level proof to perform
+     some basic manipulations that the standard Coq tactics cannot handle once
+     we hide Intermediate behind an interface. Inversion lemmas to replace
+     simple destructs and rewrites are, of course, trivial: these do not need
+     to be added to our instance's Intermediate. *)
+  Definition prog_main :=
+    @Intermediate.prog_main.
+
+  Definition prog_procedures :=
+    @Intermediate.prog_procedures.
+
+  Lemma closed_program_inv : forall p,
+    closed_program p ->
+    closed_interface (prog_interface p) /\
+    exists mainP main_procs,
+      prog_main p = Some mainP /\
+      (prog_procedures p) Component.main = Some main_procs /\
+      mainP \in domm main_procs.
+  Proof.
+    by intros p [Hclosed Hmain].
+  Qed.
+
+  Lemma closed_interface_inv : forall p1 p2,
+    closed_interface (prog_interface (program_link p1 p2)) =
+    closed_interface (unionm (prog_interface p1) (prog_interface p2)).
+  Proof.
+    easy.
+  Qed.
+End Intermediate_Instance.
+
+Module Type Source_Sig (Intermediate : Intermediate_Sig).
   Parameter program : Type.
 
   Parameter prog_interface : program -> Program.interface.
@@ -129,7 +265,7 @@ Module Type Source_Sig.
       Intermediate.well_formed_program c ->
       linkable (Intermediate.prog_interface p) (Intermediate.prog_interface c) ->
       Intermediate.closed_program (Intermediate.program_link p c) ->
-      program_behaves (I.CS.sem (Intermediate.program_link p c)) b ->
+      program_behaves (Intermediate.CS.sem (Intermediate.program_link p c)) b ->
       prefix m b ->
       not_wrong_finpref m ->
     exists p' c',
@@ -158,7 +294,7 @@ Module Type Source_Sig.
   End PS.
 End Source_Sig.
 
-Module Source_Instance <: Source_Sig.
+Module Source_Instance <: Source_Sig Intermediate_Instance.
   Definition program :=
     @Source.program.
 
@@ -203,7 +339,9 @@ Module Source_Instance <: Source_Sig.
   End PS.
 End Source_Instance.
 
-Module Type Compiler_Sig (Source : Source_Sig).
+Module Type Compiler_Sig
+       (Intermediate : Intermediate_Sig)
+       (Source : Source_Sig Intermediate).
   Parameter compile_program : Source.program -> option Intermediate.program.
 
   Axiom well_formed_compilable :
@@ -246,15 +384,16 @@ Module Type Compiler_Sig (Source : Source_Sig).
       compile_program c = Some c_comp ->
       compile_program (Source.program_link p c) = Some pc_comp ->
     forall b : program_behavior,
-      program_behaves (I.CS.sem pc_comp) b <->
-      program_behaves (I.CS.sem (Intermediate.program_link p_comp c_comp)) b.
+      program_behaves (Intermediate.CS.sem pc_comp) b <->
+      program_behaves (Intermediate.CS.sem (Intermediate.program_link p_comp c_comp)) b.
 
   Axiom I_simulates_S :
     forall p,
       Source.closed_program p ->
       Source.well_formed_program p ->
     forall tp,
-      compile_program p = Some tp -> forward_simulation (Source.CS.sem p) (I.CS.sem tp).
+      compile_program p = Some tp ->
+      forward_simulation (Source.CS.sem p) (Intermediate.CS.sem tp).
 
   Axiom S_simulates_I:
     forall p,
@@ -262,10 +401,10 @@ Module Type Compiler_Sig (Source : Source_Sig).
       Source.well_formed_program p ->
     forall tp,
       compile_program p = Some tp ->
-      backward_simulation (Source.CS.sem p) (I.CS.sem tp).
+      backward_simulation (Source.CS.sem p) (Intermediate.CS.sem tp).
 End Compiler_Sig.
 
-Module Compiler_Instance <: Compiler_Sig Source_Instance.
+Module Compiler_Instance <: Compiler_Sig Intermediate_Instance Source_Instance.
   Definition compile_program :=
     @Compiler.compile_program.
 
@@ -295,8 +434,9 @@ Module Compiler_Instance <: Compiler_Sig Source_Instance.
 End Compiler_Instance.
 
 Module RSC_DC_MD_Module
-       (Source : Source_Sig)
-       (Compiler : Compiler_Sig Source).
+       (Intermediate : Intermediate_Sig)
+       (Source : Source_Sig Intermediate)
+       (Compiler : Compiler_Sig Intermediate Source).
 Section RSC_DC_MD_Section.
 
   Variable p: Source.program.
@@ -317,7 +457,7 @@ Section RSC_DC_MD_Section.
 
   Theorem RSC_DC_MD:
     forall b m,
-      program_behaves (I.CS.sem (Intermediate.program_link p_compiled Ct)) b ->
+      program_behaves (Intermediate.CS.sem (Intermediate.program_link p_compiled Ct)) b ->
       prefix m b ->
       not_wrong b -> (* CH: could try to weaken this later to `nor_wrong m` *)
     exists Cs beh,
@@ -357,7 +497,7 @@ Section RSC_DC_MD_Section.
     { now destruct m, t; simpl; auto. }
 
     (* intermediate decomposition (for p_compiled) *)
-    pose proof Intermediate.Decomposition.decomposition_with_safe_behavior
+    pose proof Intermediate.decomposition_with_safe_behavior
       well_formed_p_compiled well_formed_Ct linkability_pcomp_Ct Hbeh Hsafe_beh as HP_decomp.
 
     (* CH: if we had undefined behavior we would use this *)
@@ -414,8 +554,8 @@ Section RSC_DC_MD_Section.
       apply Compiler.well_formed_compilable; assumption.
     }
 
-    assert (forall b, program_behaves (I.CS.sem P'_Cs_compiled) b <->
-                 program_behaves (I.CS.sem (Intermediate.program_link P'_compiled Cs_compiled)) b)
+    assert (forall b, program_behaves (Intermediate.CS.sem P'_Cs_compiled) b <->
+                      program_behaves (Intermediate.CS.sem (Intermediate.program_link P'_compiled Cs_compiled)) b)
       as HP'_Cs_behaves. {
       apply Compiler.separate_compilation_weaker with (p:=P') (c:=Cs);
         try assumption;
@@ -424,7 +564,7 @@ Section RSC_DC_MD_Section.
     have well_formed_P'Cs : Source.well_formed_program (Source.program_link P' Cs).
       rewrite -Hsame_iface1 -Hsame_iface2 in linkability_pcomp_Ct.
       exact: Source.linking_well_formedness well_formed_P' well_formed_Cs linkability_pcomp_Ct.
-    have HP'_Cs_compiled_beh : program_behaves (I.CS.sem P'_Cs_compiled) beh.
+    have HP'_Cs_compiled_beh : program_behaves (Intermediate.CS.sem P'_Cs_compiled) beh.
       have sim := Compiler.I_simulates_S HP'Cs_closed well_formed_P'Cs HP'_Cs_compiles.
       exact: (forward_simulation_same_safe_behavior sim).
 
@@ -437,7 +577,7 @@ Section RSC_DC_MD_Section.
        | assumption ].
 
     have [beh2 [HCs_decomp HCs_beh_improves]] :=
-         Intermediate.Decomposition.decomposition_with_refinement
+         Intermediate.decomposition_with_refinement
            well_formed_Cs_compiled well_formed_P'_compiled
            linkability' HP'_Cs_compiled_beh.
     have {HCs_beh_improves} ? : beh2 = beh by case: HCs_beh_improves => [<-|[? []]].
@@ -483,15 +623,21 @@ Section RSC_DC_MD_Section.
         eapply Source.linkable_disjoint_mains; assumption.
     }
 
+    (* RB: TODO: This definition needs to be transparent and does not actually rely on
+       the Intermediate interface at all! Relocate? *)
     assert (PS.mergeable_interfaces (Intermediate.prog_interface p_compiled)
                                     (Intermediate.prog_interface Cs_compiled))
       as Hmergeable_ifaces.
     {
       split.
       - assumption.
-      - by destruct HpCs_compiled_closed.
+      - apply Intermediate.closed_program_inv in HpCs_compiled_closed.
+        destruct HpCs_compiled_closed
+          as [HpCs_compiled_closed_interface HpCs_compiled_closed_main].
+        erewrite <- Intermediate.closed_interface_inv.
+        assumption.
     }
-    pose proof composition_prefix
+    pose proof Intermediate.composition_prefix
          well_formed_p_compiled well_formed_Cs_compiled
          linkable_mains linkability'' HpCs_compiled_closed
          Hmergeable_ifaces
@@ -522,8 +668,8 @@ Section RSC_DC_MD_Section.
                Compiler.compile_program (Source.program_link p Cs) = Some pCs_compiled)
       as [pCs_compiled HpCs_compiles]
       by now apply Compiler.well_formed_compilable.
-    assert (forall b, program_behaves (I.CS.sem pCs_compiled) b <->
-                 program_behaves (I.CS.sem (Intermediate.program_link p_compiled Cs_compiled)) b)
+    assert (forall b, program_behaves (Intermediate.CS.sem pCs_compiled) b <->
+                      program_behaves (Intermediate.CS.sem (Intermediate.program_link p_compiled Cs_compiled)) b)
       as HpCs_compiled_behaves
       by now apply Compiler.separate_compilation_weaker with (p:=p) (c:=Cs).
     apply HpCs_compiled_behaves in HpCs_compiled_beh.
@@ -585,7 +731,8 @@ Section RSC_DC_MD_Section.
 End RSC_DC_MD_Section.
 End RSC_DC_MD_Module.
 
-Module RSC_DC_MD_Instance := RSC_DC_MD_Module Source_Instance Compiler_Instance.
+Module RSC_DC_MD_Instance :=
+  RSC_DC_MD_Module Intermediate_Instance Source_Instance Compiler_Instance.
 
 Definition RSC_DC_MD :=
   RSC_DC_MD_Instance.RSC_DC_MD.
